Complexitylib/Models.lean
@@ -8,6 +8,7 @@ module
 public import Complexitylib.Models.TuringMachine
 public import Complexitylib.Models.TuringMachine.Oracle
 public import Complexitylib.Models.TuringMachine.Oracle.OutputSemantics
+public import Complexitylib.Models.TuringMachine.Oracle.Universality
 public import Complexitylib.Models.TuringMachine.Trace
 public import Complexitylib.Models.TuringMachine.Trace.DetPrefix
 public import Complexitylib.Models.TuringMachine.SingleTape
